{
 "cells": [
  {
   "cell_type": "markdown",
   "id": "a85a8a8b-3342-490a-b4ad-18786a214513",
   "metadata": {},
   "source": [
    "Q1 Find the val%e of T(2) for the rec%rrence relation T(n) = 3T(n-1) + 12n, given that T(0)=5."
   ]
  },
  {
   "cell_type": "markdown",
   "id": "87b03a58-2ebe-466a-9404-f7e5f1b5b5f0",
   "metadata": {},
   "source": [
    "Recurrence relation: T(n)=3T(n−1)+12n\n",
    "\n",
    "We need to find T(2), so we'll use the recurrence relation to express T(2) in terms of T(1) and \n",
    "T(1) in terms of T(0).\n",
    "\n",
    "T(2)=3T(1)+12×2\n",
    "Now, let's find \n",
    "T(1) using the same recurrence relation:\n",
    "T(1)=3T(0)+12×1\n",
    "\n",
    "Given that \n",
    "T(0)=5, we can substitute this value into the expression:\n",
    "T(1)=3×5+12×1\n",
    "\n",
    "Calculate \n",
    "T(1), and then substitute it back into the expression for \n",
    "T(2) to get the final result.\n",
    "T(2)=3×T(1)+12×2\n",
    "\n",
    "Calculate \n",
    "T(1) using the given recurrence relation:\n",
    "T(1)=3×T(0)+12×1\n",
    "\n",
    "Given that \n",
    "T(0)=5:\n",
    "T(1)=3×5+12×1=15+12=27\n",
    "\n",
    "Now that we have \n",
    "T(1), substitute it into the expression for \n",
    "T(2):\n",
    "T(2)=3×T(1)+12×2\n",
    "\n",
    "Substitute \n",
    "T(1)=27:\n",
    "T(2)=3×27+12×2=81+24=105\n",
    "\n",
    "So, the value of \n",
    "T(2) for the given recurrence relation \n",
    "T(n)=3T(n−1)+12n with the initial condition \n",
    "T(0)=5 is \n",
    "105."
   ]
  },
  {
   "cell_type": "markdown",
   "id": "8dbd38bb-71f2-49f3-a658-0b75b9b11fed",
   "metadata": {},
   "source": [
    "Q2. 2. Given a rec%rrence relation, solve it %sing the s%bstit%tion method:\n",
    "a. T(n) = T(n-1) + c\n",
    "b. T(n) = 2T(n/2) + n\n",
    "c. T(n) = 2T(n/2) + c\n",
    "d. T(n) = T(n/2) + c"
   ]
  },
  {
   "cell_type": "markdown",
   "id": "f0e6eeeb-5603-4258-827f-bffe8ac21574",
   "metadata": {},
   "source": [
    "Solutions\n",
    "\n",
    "Using substitution method for the solution:\n",
    "\n",
    "a. T(n)=T(n−1)+c\n",
    "\n",
    "Solution:\n",
    "expressing \n",
    "T(n) in terms of T(n−1) and continue until we reach the base case.\n",
    "\n",
    "T(n)=T(n−1)+c\n",
    "T(n−1)=T(n−2)+c\n",
    "T(n−2)=T(n−3)+c\n",
    "T(2)=T(1)+c\n",
    "\n",
    "T(1)=T(0)+c\n",
    "\n",
    "Now, substitute the expressions back into the original recurrence relation:\n",
    "\n",
    "T(n)=T(n−1)+c\n",
    "T(n)=(T(n−2)+c)+c\n",
    "T(n)=((T(n−3)+c)+c)+c\n",
    "...\n",
    "\n",
    "T(n)=T(1)+c⋅(n−1)\n",
    "T(n)=T(0)+c⋅n\n",
    "\n",
    "Therefore, the solution for \n",
    "\n",
    "T(n)=T(n−1)+c is T(n)=T(0)+c⋅n.\n",
    "\n",
    "\n",
    "b. T(n)=2T(n/2)+n\n",
    "\n",
    "Solution:\n",
    "Let's use the substitution method for this recurrence relation:\n",
    "T(n)=2T(n/2)+n\n",
    "\n",
    "Assume \n",
    "T(k)=ck for some constant c and all \n",
    "k<n.\n",
    "\n",
    "Now, substitute this assumption into the recurrence relation:\n",
    "T(n)=2T(n/2)+n\n",
    "\n",
    "T(n)=2c(n/2)+n\n",
    "T(n)=cn+n\n",
    "\n",
    "T(n)=(c+1)n\n",
    "\n",
    "Therefore, the solution for T(n)=2T(n/2)+n is \n",
    "\n",
    "T(n)=(c+1)n.\n",
    "\n",
    "c. \n",
    "T(n)=2T(n/2)+c\n",
    "\n",
    "Solution:\n",
    "Using the same assumption as before, \n",
    "T(k)=ck:\n",
    "\n",
    "T(n)=2T(n/2)+c\n",
    "T(n)=2c(n/2)+c\n",
    "\n",
    "T(n)=cn+c\n",
    "\n",
    "Therefore, the solution for \n",
    "T(n)=2T(n/2)+c is \n",
    "\n",
    "T(n)=cn+c.\n",
    "\n",
    "d. \n",
    "T(n)=T(n/2)+c\n",
    "\n",
    "Solution:\n",
    "Using the same assumption as before, \n",
    "T(k)=ck:\n",
    "\n",
    "T(n)=T(n/2)+c\n",
    "\n",
    "T(n)=c(n/2)+c\n",
    "T(n)=cn/2+c\n",
    "\n",
    "Therefore, the solution for \n",
    "T(n)=T(n/2)+c is T(n)=cn/2+c."
   ]
  },
  {
   "cell_type": "markdown",
   "id": "8fabdfaa-f482-4577-992c-54a45c62059d",
   "metadata": {},
   "source": [
    "3. Given a rec%rrence relation, solve it %sing the rec%rsive tree approach:\n",
    "a. T(n) = 2T(n-1) +1\n",
    "b. T(n) = 2T(n/2) + n\n",
    "\n",
    "a. T(n)=2T(n−1)+1\n",
    "\n",
    "Solution:\n",
    "For this recurrence relation, let's visualize the recursive tree:\n",
    "\n",
    "scss\n",
    "Copy code\n",
    "T(n)\n",
    "   |\n",
    "T(n-1)\n",
    "   |\n",
    "T(n-2)\n",
    "   |\n",
    " ...\n",
    "   |\n",
    "T(1)\n",
    "\n",
    "At each level, we have a cost of n because the cost is \n",
    "\n",
    "n at each node. The tree goes down to \n",
    "T(1). The total number of levels is \n",
    "log\n",
    "\n",
    "The total cost at each level is \n",
    "n, and there are n levels.\n",
    "T(n)=n+n+n+…+n=nlog2n\n",
    "\n",
    "Therefore, the solution for \n",
    "\n",
    "T(n)=2T(n/2)+n is \n",
    "T(n)=nlog2n"
   ]
  }
 ],
 "metadata": {
  "kernelspec": {
   "display_name": "Python 3 (ipykernel)",
   "language": "python",
   "name": "python3"
  },
  "language_info": {
   "codemirror_mode": {
    "name": "ipython",
    "version": 3
   },
   "file_extension": ".py",
   "mimetype": "text/x-python",
   "name": "python",
   "nbconvert_exporter": "python",
   "pygments_lexer": "ipython3",
   "version": "3.10.8"
  }
 },
 "nbformat": 4,
 "nbformat_minor": 5
}
